correctness/RegexCorrectness/Backtracker/Compile.lean
@@ -4,75 +4,59 @@ import RegexCorrectness.NFA.Semantics
 
 set_option autoImplicit false
 
-open String (Pos Iterator)
+open String (ValidPos)
 open Regex.NFA (EquivUpdate)
-open Regex.Data (CaptureGroups BitMatrix BoundedIterator)
+open Regex.Data (CaptureGroups BitMatrix BVPos)
 
 namespace Regex.Backtracker
 
 namespace captureNext
 
-theorem path_done_of_some {nfa wf it update} (hres : captureNext HistoryStrategy nfa wf it = .some update) (v : it.Valid) :
-  ∃ state it' it'', nfa[state] = .done ∧ it'.toString = it.toString ∧ it.pos ≤ it'.pos ∧ Path nfa wf it' it'' state update := by
-  let bit : BoundedIterator it.pos.byteIdx it.toString.endPos.byteIdx := ⟨it, Nat.le_refl _, v.le_endPos, rfl⟩
-  simp [captureNext_le v.le_endPos] at hres
-  have ⟨state, bit', bit'', hn, reaches, path⟩ := go.path_done_of_some (bit := bit) v hres
-  have ⟨_, _, eqs, le⟩ := BoundedIterator.Reaches.iff_valid_le_pos.mp reaches
-  simp [BoundedIterator.toString] at eqs
-  simp [BoundedIterator.pos] at le
-  exact ⟨state, bit'.it, bit''.it, hn, eqs.symm, le, path⟩
+theorem path_done_of_some {s nfa wf pos update} (hres : captureNext (HistoryStrategy s) nfa wf pos = .some update) :
+  ∃ state pos' pos'', nfa[state] = .done ∧ pos ≤ pos' ∧ Path nfa wf pos' pos'' state update := by
+  let bvpos : BVPos pos := ⟨pos, ValidPos.le_refl _⟩
+  dsimp [captureNext] at hres
+  have ⟨state, bvpos', bvpos'', hn, le, path⟩ := go.path_done_of_some hres
+  exact ⟨state, bvpos'.current, bvpos''.current, hn, le, path⟩
 
-theorem capture_of_some_compile {e it update} (hres : captureNext HistoryStrategy (NFA.compile e) NFA.compile_wf it = .some update) (v : it.Valid) :
-  ∃ it' it'' groups,
-    it'.toString = it.toString ∧
-    it.pos ≤ it'.pos ∧
-    e.Captures it' it'' groups ∧
+theorem capture_of_some_compile {s e pos update} (hres : captureNext (HistoryStrategy s) (NFA.compile e) NFA.compile_wf pos = .some update) :
+  ∃ pos' pos'' groups,
+    pos ≤ pos' ∧
+    e.Captures pos' pos'' groups ∧
     EquivUpdate groups update := by
-  have ⟨state, it', it'', hn, eqs, le, path⟩ := path_done_of_some hres v
+  have ⟨state, pos', pos'', hn, le, path⟩ := path_done_of_some hres
   have eq_zero := (NFA.done_iff_zero_compile rfl state).mp hn
   have ne : state.val ≠ (NFA.compile e).start := eq_zero ▸ Nat.ne_of_lt (NFA.lt_zero_start_compile rfl)
   have path := path.nfaPath_of_ne ne
   have ⟨groups, eqv, c⟩ := NFA.captures_of_path_compile rfl (eq_zero ▸ path.compile_liftBound rfl)
-  exact ⟨it', it'', groups, eqs, le, c, eqv⟩
+  exact ⟨pos', pos'', groups, le, c, eqv⟩
 
-theorem ne_done_of_path_of_none {nfa wf it} (hres : captureNext HistoryStrategy nfa wf it = .none) (v : it.Valid) :
-  ∀ (it' it'' : Iterator) (state : Fin nfa.nodes.size) (update : List (Nat × Pos.Raw)),
-    it'.toString = it.toString →
-    it.pos ≤ it'.pos →
-    Path nfa wf it' it'' state update →
+theorem ne_done_of_path_of_none {s nfa wf pos} (hres : captureNext (HistoryStrategy s) nfa wf pos = .none) :
+  ∀ (pos' pos'' : ValidPos s) (state : Fin nfa.nodes.size) (update : List (Nat × ValidPos s)),
+    pos ≤ pos' →
+    Path nfa wf pos' pos'' state update →
     nfa[state] ≠ .done := by
-  simp [captureNext_le v.le_endPos] at hres
+  dsimp [captureNext] at hres
 
-  let startIdx := it.pos.byteIdx
-  let maxIdx := it.toString.endPos.byteIdx
-  let bit : BoundedIterator startIdx maxIdx := ⟨it, Nat.le_refl _, v.le_endPos, rfl⟩
-  let visited := BitMatrix.zero nfa.nodes.size (maxIdx + 1 - startIdx)
+  let bvpos : BVPos pos := ⟨pos, ValidPos.le_refl _⟩
+  let visited := BitMatrix.zero nfa.nodes.size (pos.remainingBytes + 1)
 
-  have reaches : bit.Reaches bit := .refl v
-  have h := go.ne_done_of_path_of_none hres reaches go.Inv.zero captureNextAux.NotDoneInv.zero
+  have h := go.ne_done_of_path_of_none hres (BVPos.le_refl _) go.Inv.zero captureNextAux.NotDoneInv.zero
 
-  intro it' it'' state update eqs ge path hn
-  have v' : it'.Valid := path.validL
-  have v'' : it''.Valid := path.validR
-  have le' : it'.pos ≤ it.toString.endPos := eqs ▸ v'.le_endPos
-  have le'' : it''.pos ≤ it.toString.endPos := eqs ▸ path.toString_eq ▸ v''.le_endPos
-  let bit' : BoundedIterator startIdx maxIdx := ⟨it', ge, le', eqs ▸ rfl⟩
-  let bit'' : BoundedIterator startIdx maxIdx := ⟨it'', Nat.le_trans ge path.le_pos, le'', path.toString_eq ▸ eqs ▸ rfl⟩
+  intro pos' pos'' state update le path hn
+  let bvpos' : BVPos pos := ⟨pos', le⟩
+  let bvpos'' : BVPos pos := ⟨pos'', ValidPos.le_trans le path.le⟩
 
-  have reaches : bit.Reaches bit' := by
-    simp [BoundedIterator.Reaches.iff_valid_le_pos]
-    exact ⟨v, v', eqs.symm, ge⟩
+  exact h bvpos' bvpos'' state update bvpos'.le path hn
 
-  exact h bit' bit'' state update reaches path hn
-
-theorem not_captures_of_none_compile {e it} (hres : captureNext HistoryStrategy (NFA.compile e) NFA.compile_wf it = .none) (v : it.Valid)
-  (it' it'' : Iterator) (groups : CaptureGroups) (eqs : it'.toString = it.toString) (le : it.pos ≤ it'.pos) :
-  ¬e.Captures it' it'' groups := by
+theorem not_captures_of_none_compile {s e pos} (hres : captureNext (HistoryStrategy s) (NFA.compile e) NFA.compile_wf pos = .none)
+  (pos' pos'' : ValidPos s) (groups : CaptureGroups s) (le : pos ≤ pos') :
+  ¬e.Captures pos' pos'' groups := by
   intro c
   have ⟨update, _, path⟩ := NFA.path_of_captures_compile rfl c
 
   let zero : Fin (NFA.compile e).nodes.size := ⟨0, NFA.lt_zero_size_compile rfl⟩
-  have hne := ne_done_of_path_of_none hres v it' it'' zero update eqs le (Path.of_nfaPath (path.liftBound (by decide)))
+  have hne := ne_done_of_path_of_none hres pos' pos'' zero update le (Path.of_nfaPath (path.liftBound (by decide)))
   have hn := (NFA.done_iff_zero_compile (e := e) rfl zero).mpr (by simp [zero])
   exact hne hn
 
